src/transform/EliminateAlgebraic.v
@@ -1,0 +1,22 @@
+(* Require Import TermFuncs PatternComp.
+(** Compile match patterns *)
+Check t_open_branch.
+Fixpoint rewriteT (t: term_c) :=
+  match (t_node_of t) with
+  | Tcase t bl =>
+    let t1 := rewriteT t in
+    let rest := compile_bare t_case_close t_let_close_simp [t1] 
+      (map (fun b => 
+        )) 
+
+
+let rec rewriteT t0 = match t0.t_node with
+  | Tcase (t,bl) ->
+      let t = rewriteT t in
+      let mk_b b = let p,t = t_open_branch b in [p], rewriteT t in
+      let mk_case = t_case_close and mk_let = t_let_close_simp in
+      let res = Pattern.compile_bare ~mk_case ~mk_let [t] (List.map mk_b bl) in
+      t_attr_copy t0 res
+  | _ -> t_map rewriteT t0
+
+let compile_match = Trans.decl (fun d -> [decl_map rewriteT d]) None *)
